Set Cover to Hitting Set/SetModules old.dfy
@@ -192,7 +192,6 @@ lemma mult_preserves_order(a:int, b:int, a':int, b':int)
 method verifySetCover(U:Set, S:SetSet, k:nat,ghost counter_in:nat) returns (b:bool,ghost counter:nat)
 ensures b == (isCover(U.Model(),S.Model()) &&  |S.Model()| <= k)
 ensures counter <= counter_in + 2 + |U.Model()|*(U.sizeSet() + |S.Model()|*(S.maximumSizeElements() + S.sizeSetSet() + S.maximumSizeElements() + 1) + 3)
-//ensures counter <= counter_in + 2 + |U.Model()|*U.sizeSet() + |U.Model()|*(|S.Model()|*S.maximumSizeElements() + |S.Model()|*S.sizeSetSet() + |S.Model()|*S.maximumSizeElements() + |S.Model()|*1) + |U.Model()|*3
 {
   counter := counter_in;
   
@@ -329,20 +328,7 @@ ensures counter <= counter_in + 2 + |U.Model()|*(U.sizeSet() + |S.Model()|*(S.ma
   b := emptyU && b && size <= k;
 
   assert counter <= counter_in + 2 + |U.Model()|*(U.sizeSet() + |S.Model()|*(S.maximumSizeElements() + S.sizeSetSet() + S.maximumSizeElements() + 1) + 3);
-  //ghost var f1 := |S.Model()|*(S.maximumSizeElements() + S.sizeSetSet() + S.maximumSizeElements() + 1);
-  //assert counter <= counter_in + 2 + |U.Model()|*(U.sizeSet() + f1 + 3);
-  //assert counter <= counter_in + 2 + |U.Model()|*U.sizeSet() + |U.Model()|*f1 + |U.Model()|*3;
-  //ghost var f2 := (|S.Model()|*S.maximumSizeElements() + |S.Model()|*S.sizeSetSet() + |S.Model()|*S.maximumSizeElements() + |S.Model()|*1);
-  //assert f1 == f2;
-  //assert counter <= counter_in + 2 + |U.Model()|*U.sizeSet() + |U.Model()|*f2 + |U.Model()|*3;
-  //assert counter <= counter_in + 2 + |U.Model()|*U.sizeSet() + |U.Model()|*(|S.Model()|*S.maximumSizeElements() + |S.Model()|*S.sizeSetSet() + |S.Model()|*S.maximumSizeElements() + |S.Model()|*1) + |U.Model()|*3;
-  //assume false;
-  //assert |U.Model()|*((|S.Model()|*S.maximumSizeElements()) + (|S.Model()|*S.sizeSetSet()) + (|S.Model()|*S.maximumSizeElements()) + (|S.Model()|*1)) ==
-  //       |U.Model()|*(|S.Model()|*S.maximumSizeElements()) + |U.Model()|*(|S.Model()|*S.sizeSetSet()) + |U.Model()|*(|S.Model()|*S.maximumSizeElements()) + |U.Model()|*(|S.Model()|*1);
-  //assert counter <= counter_in + 2 + |U.Model()|*U.sizeSet() + |U.Model()|*|S.Model()|*S.maximumSizeElements() + |U.Model()|*|S.Model()|*S.sizeSetSet() + |U.Model()|*|S.Model()|*S.maximumSizeElements() + |U.Model()|*|S.Model()|*1 + |U.Model()|*3;
-
   assert b == (isCover(U.Model(),S.Model()) &&  |S.Model()| <= k);
-
 }
 
 
@@ -474,13 +460,170 @@ lemma SetCover_HittingSet2<T>(U:set<T>, S: set<set<T>>, k:nat)
 
 
 
-method {:verify false} method_SetCover_to_HittingSet(U:Set, S:SetSet, k: nat) returns (r:(SetSet, SetSetSet, int), ghost counter:int)
+method method_SetCover_to_HittingSet(U:Set, S:SetSet, k: nat) returns (r:(set<set<T>>, set<set<set<T>>>, int), ghost counter:int)
   requires forall s | s in S.Model() :: s <= U.Model()
   requires isCover(U.Model(), S.Model())
-  //ensures r == SetCover_to_HittingSet(U.Model(), S.Model(), k)
+  ensures r == SetCover_to_HittingSet(U.Model(), S.Model(), k)
   //ensures counter <= 2*|U| + 2*|S|*|S|*|U| + |S|*|U|*|U| + 2*|S|*|U| + 3*|U|*|U|
 {
-  // ...
+  assert |U.Model()| >= 0 && |S.Model()| >= 0;
+
+  ghost var sizeT:int := 1;
+  counter := 0;
+
+  var HU := S;
+  var Hk := k;
+
+  var HS:set<set<set<T>>> := {};
+  var U2 := U;
+
+  while 0<|U2.Model()|
+    decreases U2
+    
+    invariant forall s | s in HS :: s <= HU.Model()
+    invariant HS == (set u | u in (U.Model() - U2.Model()) :: (set s | s in S.Model() && u in s))
+    
+    invariant |HS| <= |U.Model() - U2.Model()|
+    invariant counter <= ((2 + (2*|S.Model()| + |U.Model()| + 2)*(|S.Model()|))  + 3*|U.Model()|) * |U.Model() - U2.Model()|
+
+    //invariant |U| >= 0 && |S| >= 0
+  {
+
+    ghost var prevDifference := |U.Model() - U2.Model()|;
+    ghost var prevCounter := counter;
+    counter := counter + 1;
+    //var v :| v in U2;
+    var v;
+    v, counter := U2.Pick(counter);
+    assert counter == prevCounter + 2;
+
+    var S2 := S;
+    //assert counter == prevCounter + 2 + (1 + |U| + |S|*|U| + |U| + |S|*|U|)*(|S| - |S2|);
+    var hs:SetSet, counter := NewSetSet(counter);
+
+    while 0<|S2.Model()|
+      decreases S2
+
+      invariant hs.Model() == (set s | s in (S.Model() - S2.Model()) && v in s)
+      invariant HS == (set u | u in (U.Model() - U2.Model()) :: (set s | s in S.Model() && u in s))
+
+      invariant forall s | s in S2.Model() :: s <= U.Model()
+      invariant S2.Model() <= S.Model()
+      invariant hs.Model() <= S.Model()
+
+      //invariant counter <= prevCounter + 2 + (1 + |U| + |S|*|U| + |U| + |S|*|U|)*(|S| - |S2|)
+    {
+      //ghost var increment := 1 + |U| + |S|*|U| + |U| + |S|*|U|;
+      //assert 1 + |U| + |S|*|U| + |U| + |S|*|U| == increment;
+
+      ghost var counter_iteration_loop := counter;
+      ghost var prev_S_minus_S2 := |S.Model()| - |S2.Model()|;
+
+      counter := counter + 1;
+      //var s :| s in S2;
+      var s:Set;
+      s, counter := S2.Pick(counter);        // |U|
+      assert counter <= counter_iteration_loop + 1 + |U.Model()|;
+
+      if_subset_then_smaller(s.Model(), U.Model());
+      if_subset_then_smaller(S2.Model(), S.Model());
+
+      assert |S.Model()| - |S2.Model()| == prev_S_minus_S2;
+      //S2 := S2 - {s};
+      S2, counter := S2.Remove(s, counter);  // |S|*|U|
+      //assert counter <= counter_iteration_loop + 1 + |U| + |S|*|U|;
+
+      //assert |S| - |S2| == prev_S_minus_S2 + 1;
+
+      var cont:bool;
+      cont, counter := s.Contains(v, counter);  // |U|
+      //assert counter <= counter_iteration_loop + 1 + |U| + |S|*|U| + |U|;
+      if (cont == true) { //v in s {
+        //hs := hs + {s};
+        assert s.Model() in S.Model();
+        hs, counter := hs.Add(s, counter);  // |S|*|U|
+        assert hs.Model() <= S.Model();
+        if_subset_then_smaller(hs.Model(), S.Model());
+      }
+      
+      //assert counter <= prevCounter + 2 + (1 + |U| + |S|*|U| + |U| + |S|*|U|)*(|S| - |S2|)
+      //by {
+      //  assert counter <= counter_iteration_loop + 1 + |U| + |S|*|U| + |U| + |S|*|U|;
+      //  assert counter <= counter_iteration_loop + increment;
+
+      //  assert hs == (set s | s in (S - S2) && v in s);
+      // assert HS == (set u | u in (U - U2) :: (set s | s in S && u in s));
+
+      //  assert forall s | s in S2 :: s <= U;
+      //  assert S2 <= S;
+      //  assert hs <= S;
+
+      //  assert counter_iteration_loop <= prevCounter + 2 + (increment)*prev_S_minus_S2;
+      //  assert |S| - |S2| == prev_S_minus_S2 + 1;
+
+      //  assert counter <= prevCounter + 2 + (increment)*prev_S_minus_S2 + increment;
+      //  assert counter <= prevCounter + 2 + (increment)*(prev_S_minus_S2 + 1);
+      //}
+    }
+  
+    //assert counter <= prevCounter + 2 + (1 + |U| + |S|*|U| + |U| + |S|*|U|)*(|S|);
+    
+    //HS := HS + {hs};
+    ghost var prevHS := HS;
+    HS, counter := SetMod.add(HS, hs, |U|*|S|, counter);
+    assert |HS| <= |prevHS| + 1;
+
+
+    assert |HS| <= |U|;
+    assert |U| >= 0 && |S| >= 0;
+    //assert 0 <= |U|;
+    //assert 0 <= |S|*|U|;
+    assert |HS|*(|U|*|S|) <= |U|*(|U|*|S|);
+
+    assert counter <= prevCounter + 2 + (1 + |U| + |S|*|U| + |U| + |S|*|U|)*(|S|) + |U|*|U|*|S|;
+    
+    assume false;
+
+    ghost var U3 := U2;
+    //U2 := U2 - {v};
+    U2, counter := SetMod.remove(U2, v, 1, counter);
+    assert hs == (set s | s in (S - S2) && v in s);
+    assert prevHS == (set u | u in (U - U3) :: (set s | s in S && u in s));
+    assert (U - (U2 + {v})) == (U - U3);
+    assert prevHS + {hs} == (set u | u in (U - (U2 + {v})) :: (set s | s in S && u in s)) + {(set s | s in (S - S2) && v in s)};
+
+    assert forall s | s in S2 :: !(v in s);
+
+    if_S2_has_no_set_with_v_then_can_remove_safely(S, S2, v);
+    assert {(set s | s in S && v in s)} == {(set s | s in (S - S2) && v in s)};
+
+    assert (set u | u in {v} :: (set s | s in S && u in s)) == {(set s | s in (S - S2) && v in s)};
+
+    assert (set u | u in (U - (U2 + {v})) :: (set s | s in S && u in s))
+            + (set u | u in {v} :: (set s | s in S && u in s))
+            == (set u | u in (U - (U2 + {v})) + {v} :: (set s | s in S && u in s));
+    assert (U - (U2 + {v})) + {v} == (U - U2 + {v});
+
+    assert prevHS + {hs} == (set u | u in (U - U2) :: (set s | s in S && u in s));
+    
+  }
+  assert counter <= 2*|U| + 2*|S|*|S|*|U| + |S|*|U|*|U| + 2*|S|*|U| + 3*|U|*|U|;
+
+  r := (HU, HS, Hk);
+  assert r == (HU, HS, Hk);
+
+  ghost var e := SetCover_to_HittingSet<T>(U, S, k);
+  assert HU == e.0;
+  assert Hk == e.2;
+
+  assert HS == (set u | u in (U - U2) :: (set s | s in S && u in s));
+  assert U2 == {};
+  assert (U - {}) == U;
+  assert HS == (set u | u in U :: (set s | s in S && u in s));
+
+  assert HS == e.1;
+
+  assert r == SetCover_to_HittingSet<T>(U, S, k);
 }
 
 
